Make progress on some of the hashmap proofs

tests/lean/Hashmap/Properties.lean
@@ -3,6 +3,18 @@ import Hashmap.Funs
 open Primitives
 open Result
 
+namespace List
+
+-- TODO: we don't want to use the original List.lookup because it uses BEq
+-- TODO: rewrite rule: match x == y with ... -> if x = y then ... else ... ?
+@[simp]
+def lookup' {α : Type} (ls: _root_.List (Usize × α)) (key: Usize) : Option α :=
+  match ls with
+  | [] => none
+  | (k, x) :: tl => if k = key then some x else lookup' tl key
+
+end List
+
 namespace hashmap
 
 namespace List
@@ -12,10 +24,15 @@ def v {α : Type} (ls: List α) : _root_.List (Usize × α) :=
   | Nil => []
   | Cons k x tl => (k, x) :: v tl
 
-def lookup {α : Type} (ls: _root_.List (Usize × α)) (key: Usize) : Option α :=
-  match ls with
-  | [] => none
-  | (k, x) :: tl => if k = key then some x else lookup tl key
+@[simp] theorem v_nil (α : Type) : (Nil : List α).v = [] := by rfl
+@[simp] theorem v_cons {α : Type} k x (tl: List α) : (Cons k x tl).v = (k, x) :: v tl := by rfl
+
+@[simp]
+abbrev lookup {α : Type} (ls: List α) (key: Usize) : Option α :=
+  ls.v.lookup' key
+
+@[simp]
+abbrev len {α : Type} (ls : List α) : Int := ls.v.len
 
 end List
 
@@ -23,39 +40,51 @@ namespace HashMap
 
 abbrev Core.List := _root_.List
 
+namespace List
+
+end List
+
+-- TODO: move
+@[simp] theorem neq_imp_nbeq [BEq α] [LawfulBEq α] (x y : α) (heq : ¬ x = y) : ¬ x == y := by simp [*]
+@[simp] theorem neq_imp_nbeq_rev [BEq α] [LawfulBEq α] (x y : α) (heq : ¬ x = y) : ¬ y == x := by simp [*]
+
+-- TODO: move
+theorem match_lawful_beq [BEq α] [LawfulBEq α] [DecidableEq α] (x y : α) :
+  (x == y) = (if x = y then true else false) := by
+  split <;> simp_all
+
 theorem insert_in_list_spec0 {α : Type} (key: Usize) (value: α) (ls: List α) :
   ∃ b,
     insert_in_list α key value ls = ret b ∧
-    (b ↔ List.lookup ls.v key = none)
+    (b ↔ ls.lookup key = none)
   := match ls with
-  | .Nil => by simp [insert_in_list, insert_in_list_loop, List.lookup]
+  | .Nil => by simp [insert_in_list, insert_in_list_loop]
   | .Cons k v tl =>
     if h: k = key then -- TODO: The order of k/key matters
       by
-        simp [insert_in_list, List.lookup]
+        simp [insert_in_list]
         rw [insert_in_list_loop]
         simp [h]
     else
       have ⟨ b, hi ⟩ := insert_in_list_spec0 key value tl
       by
         exists b
-        simp [insert_in_list, List.lookup]
+        simp [insert_in_list]
         rw [insert_in_list_loop] -- TODO: Using simp leads to infinite recursion
-        simp [h]
-        simp [insert_in_list] at hi
-        exact hi
+        simp only [insert_in_list] at hi
+        simp [*]
 
 -- Variation: use progress
 theorem insert_in_list_spec1 {α : Type} (key: Usize) (value: α) (ls: List α) :
   ∃ b,
     insert_in_list α key value ls = ret b ∧
-    (b ↔ List.lookup ls.v key = none)
+    (b ↔ ls.lookup key = none)
   := match ls with
-  | .Nil => by simp [insert_in_list, insert_in_list_loop, List.lookup]
+  | .Nil => by simp [insert_in_list, insert_in_list_loop]
   | .Cons k v tl =>
     if h: k = key then -- TODO: The order of k/key matters
       by
-        simp [insert_in_list, List.lookup]
+        simp [insert_in_list]
         rw [insert_in_list_loop]
         simp [h]
     else
@@ -66,19 +95,17 @@ theorem insert_in_list_spec1 {α : Type} (key: Usize) (value: α) (ls: List α) 
         progress keep as heq as ⟨ b hi ⟩
         simp only [insert_in_list] at heq
         exists b
-        simp only [heq, hi]
-        simp [*, List.lookup]
 
 -- Variation: use tactics from the beginning
 theorem insert_in_list_spec2 {α : Type} (key: Usize) (value: α) (ls: List α) :
   ∃ b,
     insert_in_list α key value ls = ret b ∧
-    (b ↔ (List.lookup ls.v key = none))
+    (b ↔ (ls.lookup key = none))
   := by
   induction ls
-  case Nil => simp [insert_in_list, insert_in_list_loop, List.lookup]
+  case Nil => simp [insert_in_list, insert_in_list_loop]
   case Cons k v tl ih =>
-    simp only [insert_in_list, List.lookup]
+    simp only [insert_in_list]
     rw [insert_in_list_loop]
     simp only
     if h: k = key then
@@ -94,26 +121,27 @@ theorem insert_in_list_back_spec {α : Type} (key: Usize) (value: α) (l0: List 
   ∃ l1,
     insert_in_list_back α key value l0 = ret l1 ∧
     -- We update the binding
-    List.lookup l1.v key = value ∧
-    (∀ k, k ≠ key → List.lookup l1.v k = List.lookup l0.v k)
+    l1.lookup key = value ∧
+    (∀ k, k ≠ key → l1.lookup k = l0.lookup k)
   := match l0 with
-  | .Nil => by simp [insert_in_list_back, insert_in_list_loop_back, List.lookup]; tauto
+  | .Nil => by
+    simp (config := {contextual := true}) [insert_in_list_back, insert_in_list_loop_back]
   | .Cons k v tl =>
      if h: k = key then
        by
-         simp [insert_in_list_back, List.lookup]
+         simp [insert_in_list_back]
          rw [insert_in_list_loop_back]
-         simp [h, List.lookup]
+         simp [h]
          intro k1 h1
          simp [*]
      else
        by
-         simp [insert_in_list_back, List.lookup]
+         simp [insert_in_list_back]
          rw [insert_in_list_loop_back]
-         simp [h, List.lookup]
+         simp [h]
          progress keep as heq as ⟨ tl hp1 hp2 ⟩
          simp [insert_in_list_back] at heq
-         simp (config := {contextual := true}) [*, List.lookup]
+         simp (config := {contextual := true}) [*]
 
 def distinct_keys (ls : Core.List (Usize × α)) := ls.pairwise_rel (λ x y => x.fst ≠ y.fst)
 
@@ -132,44 +160,103 @@ def slot_s_inv (l i : Int) (ls : Core.List (Usize × α)) : Prop :=
 
 def slot_t_inv (l i : Int) (s : List α) : Prop := slot_s_inv l i s.v
 
-@[pspec]
-theorem insert_in_list_back_spec1 {α : Type} (l : Int) (key: Usize) (value: α) (l0: List α)
+theorem insert_in_list_back_spec_aux {α : Type} (l : Int) (key: Usize) (value: α) (l0: List α)
   (hinv : slot_s_inv_hash l (hash_mod_key key l) l0.v) :
   ∃ l1,
     insert_in_list_back α key value l0 = ret l1 ∧
     -- We update the binding
-    List.lookup l1.v key = value ∧
-    (∀ k, k ≠ key → List.lookup l1.v k = List.lookup l0.v k) ∧
+    l1.lookup key = value ∧
+    (∀ k, k ≠ key → l1.lookup k = l0.lookup k) ∧
     -- We preserve part of the key invariant
-    slot_s_inv_hash l (hash_mod_key key l) l1.v
+    slot_s_inv_hash l (hash_mod_key key l) l1.v ∧
+    -- Reasoning about the length
+    match l0.lookup key with
+    | none => l1.len = l0.len + 1
+    | some _ => l1.len = l0.len
   := match l0 with
   | .Nil => by
-    simp [insert_in_list_back, insert_in_list_loop_back, List.lookup, List.v, slot_s_inv_hash]
-    tauto
+    simp (config := {contextual := true}) [insert_in_list_back, insert_in_list_loop_back, List.v, slot_s_inv_hash]
   | .Cons k v tl0 =>
      if h: k = key then
        by
-         simp [insert_in_list_back, List.lookup]
+         simp [insert_in_list_back]
          rw [insert_in_list_loop_back]
-         simp [h, List.lookup]
+         simp [h]
          constructor
          . intros; simp [*]
          . simp [List.v, slot_s_inv_hash] at *
            simp [*]
      else
        by
-         simp [insert_in_list_back, List.lookup]
+         simp [insert_in_list_back]
          rw [insert_in_list_loop_back]
-         simp [h, List.lookup]
+         simp [h]
          have : slot_s_inv_hash l (hash_mod_key key l) (List.v tl0) := by
            simp_all [List.v, slot_s_inv_hash]
-         progress keep as heq as ⟨ tl1 hp1 hp2 hp3 ⟩
+         progress keep as heq as ⟨ tl1 hp1 hp2 hp3 hp4 ⟩
          simp only [insert_in_list_back] at heq
          have : slot_s_inv_hash l (hash_mod_key key l) (List.v (List.Cons k v tl1)) := by
            simp [List.v, slot_s_inv_hash] at *
            simp [*]
-         simp (config := {contextual := true}) [*, List.lookup]
+         -- TODO: canonize addition by default?
+         simp_all [Int.add_assoc, Int.add_comm, Int.add_left_comm]
 
+theorem insert_in_list_back_spec_aux1 {α : Type} (l : Int) (key: Usize) (value: α) (l0: List α)
+  (hinv : slot_s_inv_hash l (hash_mod_key key l) l0.v)
+  (hdk : distinct_keys l0.v) :
+  ∃ l1,
+    insert_in_list_back α key value l0 = ret l1 ∧
+    -- We update the binding
+    l1.lookup key = value ∧
+    (∀ k, k ≠ key → l1.lookup k = l0.lookup k) ∧
+    -- We preserve part of the key invariant
+    slot_s_inv_hash l (hash_mod_key key l) l1.v ∧
+    -- Reasoning about the length
+    (match l0.lookup key with
+     | none => l1.len = l0.len + 1
+     | some _ => l1.len = l0.len) ∧
+    -- The keys are distinct
+    distinct_keys l1.v ∧
+    -- We need this auxiliary property to prove that the keys distinct properties is preserved
+    (∀ k, k ≠ key → l0.v.allP (λ (k1, _) => k ≠ k1) → l1.v.allP (λ (k1, _) => k ≠ k1))
+  := match l0 with
+  | .Nil => by
+    simp (config := {contextual := true})
+      [insert_in_list_back, insert_in_list_loop_back,
+       List.v, slot_s_inv_hash, distinct_keys, List.pairwise_rel]
+  | .Cons k v tl0 =>
+     if h: k = key then
+       by
+         simp [insert_in_list_back]
+         rw [insert_in_list_loop_back]
+         simp [h]
+         split_target_conjs
+         . intros; simp [*]
+         . simp [List.v, slot_s_inv_hash] at *
+           simp [*]
+         . simp [*, distinct_keys] at *
+           apply hdk
+         . tauto
+     else
+       by
+         simp [insert_in_list_back]
+         rw [insert_in_list_loop_back]
+         simp [h]
+         have : slot_s_inv_hash l (hash_mod_key key l) (List.v tl0) := by
+           simp_all [List.v, slot_s_inv_hash]
+         have : distinct_keys (List.v tl0) := by
+           simp [distinct_keys] at hdk
+           simp [hdk, distinct_keys]
+         progress keep as heq as ⟨ tl1 hp1 hp2 hp3 hp4 hp5 hp6 ⟩ -- TODO: naming is weird
+         simp only [insert_in_list_back] at heq
+         have : slot_s_inv_hash l (hash_mod_key key l) (List.v (List.Cons k v tl1)) := by
+           simp [List.v, slot_s_inv_hash] at *
+           simp [*]
+         have : distinct_keys ((k, v) :: List.v tl1) := by
+           simp [distinct_keys] at *
+           simp [*]
+         -- TODO: canonize addition by default?
+         simp_all [Int.add_assoc, Int.add_comm, Int.add_left_comm]
 
 end HashMap
 
